core/LoopWithIte.v
@@ -1,0 +1,364 @@
+Require Import Program List ZArith Arith.
+
+Set Implicit Arguments.
+
+Import Notations.
+
+Section monads.
+
+Local Notation "f ∘ g" := (fun x => f (g x)) (at level 40, left associativity).
+
+(* State Monad *)
+
+(* Record St : Type:= {
+  r : nat;
+}. *)
+
+Variable Internal_S : Type.
+
+Record St : Type := {
+  state : Internal_S ;
+  it_loop : nat
+}.
+
+Definition State (A : Type) := St -> A * St.
+
+(* Arguments State [ A ]. *)
+
+(* forall {A}, A -> m A; *)
+Definition state_pure A (a : A) : State A := 
+  fun s => (a,s).
+
+(* state_bind = 
+fun (A : Type) (st_a : State A) (B : Type) (f : A -> State B) (s : S) => let (a, s0) := st_a s in f a s0
+     : forall A : Type, State A -> forall B : Type, (A -> State B) -> S -> B * S *)
+Definition state_bind {A B} (st_a : State A) (f : A -> State B)  : State B :=
+  fun s => let (a, s0) := st_a s in f a s0.
+
+
+(*    bind: forall {A}, m A -> forall {B}, (A -> m B) -> m B;
+  bind_right_unit: forall A (a: m A), a = bind a return_;
+  bind_left_unit: forall A (a: A) B (f: A -> m B),
+             f a = bind (return_ a) f;
+  bind_associativity: forall A (ma: m A) B f C (g: B -> m C),
+                 bind ma (fun  x=> bind (f x) g) = bind (bind ma f) g *)
+(* Lemma bind_right_unit *)
+
+Lemma state_bind_right_unit : 
+  forall (A : Type) (a: State A), a = state_bind a (@ state_pure A).
+  Proof.
+  intros.
+  unfold state_bind.
+  apply functional_extensionality.
+  intros.
+  destruct (a x).
+  reflexivity.
+  Qed.
+
+Lemma state_bind_left_unit :
+   forall A (a: A) B (f: A -> State B),
+             f a = state_bind (state_pure a) f.
+   Proof.
+   auto.
+   Qed.
+
+Lemma state_bind_associativity :
+  forall A (ma: State A) B f C (g: B -> State C),
+                 state_bind ma (fun x => state_bind (f x) g) = state_bind (state_bind ma f) g.
+  Proof.
+  intros.
+  unfold state_bind.
+  apply functional_extensionality.
+  intros.
+  destruct (ma x).
+  reflexivity.
+  Qed.
+
+Definition put (x : St) : State () :=
+  fun _ => (tt,x).
+
+Definition get : State St :=
+  fun x => (x,x).
+
+Definition runState  {A} (op : State A) : St -> A * St := op.
+Definition evalState {A} (op : State A) : St -> A := fst ∘ op.
+Definition execState {A} (op : State A) : St -> St := snd ∘ op.
+
+Notation "m1 ;; m2" := (state_bind m1 (fun _ => m2))  (at level 60, right associativity) : monad_scope.
+Notation "'perf' x '<-' m ';' e" := (state_bind m (fun x => e))
+  (at level 60, x ident, m at level 200, e at level 60) : monad_scope.
+
+Open Scope monad_scope.
+
+(* modify = 
+fun (S : Type) (f : S -> S) => perf s <- getS (S:=S); putS (f s)
+     : forall S : Type, (S -> S) -> State S () *)
+Definition modify (f : St -> St) : State () :=
+  perf s <- get; put (f s).
+
+Definition s_modify (f : Internal_S -> Internal_S) : State () :=
+  modify (fun s => {| state := f (state s) ; it_loop := (it_loop s)|}).
+
+Definition Assertion := St -> Prop.
+
+Definition hoareTripleS {A} (P : St -> Prop) (m : State A) (Q : A -> St -> Prop) : Prop :=
+  forall (s : St), P s -> let (a, s') := m s in Q a s'.
+
+Notation "{{ P }} m {{ Q }}" := (hoareTripleS P m Q)
+  (at level 90, format "'[' '[' {{  P  }}  ']' '/  ' '[' m ']' '['  {{  Q  }} ']' ']'") : monad_scope.
+
+Lemma ret  (A : Type) (a : A) (P : A -> Assertion) : {{ P a }} state_pure a {{ P }}.
+Proof.
+intros s H; trivial.
+Qed.
+
+(* Triplet de hoare sur la séquence *)
+Lemma bind  (A B : Type) (m : State A) (f : A -> State B) (P : Assertion)( Q : A -> Assertion) (R : B -> Assertion) :
+  (forall a, {{ Q a }} f a {{ R }}) -> {{ P }} m {{ Q }} -> {{ P }} perf x <- m ; f x {{ R }}.
+Proof. 
+intros H1 H2 s H3.
+unfold state_bind.
+case_eq (m s).
+intros a s' H4.
+apply H2 in H3.
+rewrite H4 in H3.
+apply H1.
+apply H3.
+Qed.
+
+Definition wp {A : Type} (P : A -> St -> Prop) (m : State A) :=
+  fun s => let (a,s') := m s in P a s'.
+
+Lemma wpIsPrecondition {A : Type} (P : A -> St -> Prop) (m : State A) :
+  {{ wp P m }} m {{ P }}.
+  Proof.
+  unfold wp.
+  congruence.
+  Qed.
+
+Lemma wpIsWeakestPrecondition
+  (A : Type) (P : A -> St -> Prop) (Q : St -> Prop) (m : State A) :
+  {{ Q }} m {{ P }} -> forall s, Q s -> (wp P m) s.
+  Proof.
+  trivial.
+  Qed.
+
+Lemma assoc (A B C : Type)(m : State A)(f : A -> State B)(g : B -> State C) :
+  perf y <-
+    perf x <- m ;
+    f x ;
+  g y =
+  perf x <- m ;
+  perf y <- f x ;
+  g y.
+  Proof.
+  extensionality s; unfold state_bind; case (m s); trivial; tauto.
+  Qed.
+
+Lemma l_put (s : St) (P : unit -> Assertion) : {{ fun _ => P tt s }} put s {{ P }}.
+Proof.
+intros s0 H;trivial.
+Qed.
+
+Lemma l_get (P : St -> Assertion) : {{ fun s => P s s }} get {{ P }}.
+Proof.
+intros s H; trivial.
+Qed.
+
+Lemma bindRev (A B : Type) (m : State A) (f : A -> State B) (P : Assertion)( Q : A -> Assertion) (R : B -> Assertion) :
+  {{ P }} m {{ Q }} -> (forall a, {{ Q a }} f a {{ R }}) -> {{ P }} perf x <- m ; f x {{ R }}.
+Proof.
+intros; eapply bind ; eassumption.
+Qed.
+
+Lemma weaken (A : Type) (m : State A) (P Q : Assertion) (R : A -> Assertion) :
+  {{ Q }} m {{ R }} -> (forall s, P s -> Q s) -> {{ P }} m {{ R }}.
+Proof.
+intros H1 H2 s H3.
+apply H2 in H3. 
+apply H1 in H3.
+assumption. 
+Qed.
+
+Lemma strengthen (A : Type) (m : State A) (P: Assertion) (Q R: A -> Assertion) :
+  {{ P }} m {{ R }} -> (forall s a, R a s -> Q a s) -> {{ P }} m {{ Q }}.
+Proof.
+intros H1 H2 s H3.
+apply H1 in H3.
+Admitted.
+
+
+Lemma l_modify f (P : () -> Assertion) : {{ fun s => P tt (f s) }} modify f {{ P }}.
+Proof.
+unfold modify.
+eapply bind.
+intros.
+eapply l_put.
+simpl.
+eapply weaken.
+eapply l_get.
+intros. simpl.
+assumption.
+Qed.
+
+Definition state_liftM {A B} (f : A -> B) (ma : State A) : State B :=
+  state_bind ma (fun a => state_pure (f a)).
+  
+(* Section Continuation. *)
+
+(* Inductive Action : Type :=
+  | Atom : State Action -> Action
+  | Stop : Action.
+
+Definition LoopT a : Type := (a -> Action) -> Action.
+
+Definition loopT_pure {A} (a : A) : LoopT A :=
+  fun (c : A -> Action) => c a.
+
+Definition loopT_bind {A} (x : LoopT A) {B} (k : A -> LoopT B) : LoopT B :=
+  fun (c : B -> Action) => x (fun a => (k a) c).
+
+Definition action {A} (x : LoopT A) : Action :=
+  x (fun (_ : A) => Stop).
+
+(* lift *)
+Definition atom {A} (x : State A) : LoopT A := 
+  fun c => Atom ( perf a <- x ; state_pure (c a)).
+
+Open Scope list_scope.
+
+Fixpoint round (lst : list Action) : State () :=
+  match lst with
+    | nil => state_pure tt
+    | (a::ax) => match a with 
+                  | Atom am => am ;; round ax
+                  | Stop => round ax
+                  end
+    end.
+
+Definition run {A} (x : LoopT A) : State () :=
+  round [action x].
+
+Definition stop {A} : LoopT A :=
+  fun c => Stop. *)
+
+Inductive Action (A : Type) : Type :=
+  | Break : Action A
+  | Atom : A -> Action A.
+
+(* Definition hoareTripleS {A} (P : St -> Prop) (m : State A) (Q : A -> St -> Prop) : Prop :=
+  forall (s : St), P s -> let (a, s') := m s in Q a s'. *)
+
+Lemma act_ret  (A : Type) (a : A) (P : Assertion) : {{P}} state_pure (Atom a) 
+{{fun (_ : Action A) =>  P }}.
+Proof.
+intros s H; trivial.
+Qed.
+
+(* Lemma ret_tt (P : () -> Assertion) : {{ P tt }} state_pure tt {{ P }}.
+Proof.
+intros s H; trivial.
+Qed. *)
+
+Arguments Atom [A] _.
+Arguments Break [A].
+
+Definition LoopT a : Type := State (Action a).
+
+Definition runLoopT {A} (loop : LoopT A) : State (Action A) :=
+  loop.
+
+Definition loopT_pure {A} (a : A) : LoopT A :=
+  (state_pure (Atom a)).
+
+Definition loopT_bind  {A} (x : LoopT A) {B} (k : A -> LoopT B) : LoopT B :=
+    perf o <- runLoopT x;
+    match o with 
+      | Break => state_pure Break
+      | Atom y => runLoopT (k y)
+    end.
+
+Definition loopT_liftT {A} (a : State A) : LoopT A :=
+  state_liftM (@Atom A) a.
+
+Definition break {A} : LoopT A :=
+  state_pure Break.
+
+Definition getIt : State nat :=
+  perf s <- get ;
+  state_pure (it_loop s).
+
+Definition decrementsIt : State unit :=
+  modify (fun s => {| state := s.(state) ; it_loop := s.(it_loop) - 1 |}).
+
+Program Fixpoint foreach (it min : nat) (body : nat -> LoopT ()) : State () :=
+  perf it2 <- getIt ; 
+  if (Nat.leb it2 min) then state_pure tt
+  else match it with
+        | S it' => perf out <- runLoopT (body it);
+                               decrementsIt ;;
+                                match out with
+                                  | Break => state_pure tt
+                                  | _ => foreach it' min body
+                                end
+        | 0 => state_pure tt
+       end.
+
+Lemma foreach_rule (min max : nat) (P : St -> Prop) (body : nat -> State ())
+  : (forall (it : nat), {{fun s => P s /\ (min <= it <= max)}} body it {{fun _ => P}}) -> 
+    {{P}} foreach max min (fun it0 => loopT_liftT (body it0)) {{fun _ => P}}.
+  Proof.
+  intros H.
+  induction max.
+  + intros st HP. auto.
+  + unfold foreach.
+    case_eq (S max <=? min);intros Hm.
+    - intros s HP. trivial.
+    - eapply bindRev .
+      unfold runLoopT.
+      unfold loopT_liftT.
+      unfold state_liftM.
+      eapply bindRev.
+      * unfold hoareTripleS in H.
+        intros st H2.
+        eapply H;split;auto.
+        split;auto.
+        apply Nat.leb_gt in Hm.
+        apply Nat.lt_le_incl.
+        auto.
+      * intros [].
+        apply act_ret.
+    * intros []. intros s HP. trivial.
+      apply IHmax.
+         ++ intros it s'.
+            intros [H1 [H2 H3]].
+            apply H.
+            split;auto.
+     Qed.
+
+Lemma foreach_break_rule (min max : nat) (P : St -> Prop) (body : nat -> State ())
+  : forall (cond : bool), (forall (it : nat), {{fun s => P s /\ (min <= it <= max) /\ (cond = true) }} body it {{fun _ => P}}) -> 
+    {{P}} foreach max min (fun it0 => if (cond) then break else loopT_liftT (body it0)) {{fun _ s => P s /\ cond = false}}.
+  Admitted.
+
+Notation "'for' i '=' max 'to' min '{{' body }}" := (foreach max min (fun i => (loopT_liftT body))) (at level 60, i ident, min at level 60,
+max at level 60, body at level 60, right associativity) : monad_scope.
+
+(* (* Notation "'for_e' i '=' min 'to' max '{{' body }}" := (foreach min max (fun i => (body))) (at level 60, i ident, min at level 60,
+max at level 60, body at level 60, right associativity) : monad_scope. *)
+
+(* Notation "'for2' i '=' min 'to' max '{{' body }}" := (foreach min max (fun i => (body))) (at level 60, i ident, min at level 60,
+max at level 60, body at level 60, right associativity) : monad_scope. *) *)
+
+End monads.
+
+Notation "m1 ;; m2" := (state_bind m1 (fun _ => m2))  (at level 60, right associativity) : monad_scope.
+Notation "'perf' x '<-' m ';' e" := (state_bind m (fun x => e))
+  (at level 60, x ident, m at level 200, e at level 60) : monad_scope.
+Notation "{{ P }} m {{ Q }}" := (hoareTripleS P m Q)
+(at level 90, format "'[' '[' {{  P  }}  ']' '/  ' '[' m ']' '['  {{  Q  }} ']' ']'") : monad_scope.
+Notation "'for' i '=' max 'to' min '{{' body }}" := (foreach max min (fun i => (loopT_liftT body))) (at level 60, i ident, min at level 60,
+max at level 60, body at level 60, right associativity) : monad_scope.
+
+Open Scope monad_scope.
+
