core/TestLoop.v
@@ -1,0 +1,207 @@
+Require Import LoopV2 Program List ZArith Arith.
+
+Section ResNat.
+
+Record MySt : Type:= {
+  r : nat;
+}. 
+
+Definition init_state : MySt := {|r := 1|}.
+
+Definition add_s (i : nat) : State MySt unit :=
+  modify (fun s => {| r := s.(r) + i |}).
+
+Definition min_s (i : nat) : State MySt unit :=
+modify (fun s => {| r := s.(r) - i |}).
+
+Definition mul_s (i : nat) : State MySt unit :=
+  modify (fun s => {| r := s.(r) * i |}).
+
+(* Definition fac5 : State unit :=
+  for i = 5 to 0 {{
+    mul_s i
+  }}.
+ *)
+(* Compute runState fac5 init_state.  *)
+
+(* Definition test_exit : State () :=
+   for_e i = 0 to 20 {{
+    if (i =? 5) then break
+    else (loopT_liftT (add_s 1))
+  }}.
+ *)
+(* Compute runState test_exit init_state.  *)
+
+(* in_seq: forall len start n : nat, In n (seq start len) <-> start <= n < start + len *)
+
+
+(* Lemma foreach_break_rule_2 (min max : nat) (P : () -> St -> Prop) (body : nat -> State ()) (compare : State bool)
+  : forall (cond : bool), (forall (it : nat), {{fun s => P tt s /\ (min <= it <= max) /\ (cond s = true) }} body it {{P}}) -> 
+    {{P tt}} foreach max min (fun it0 => perf cond <- compare;  if (fun s => cond s) then break else loopT_liftT (body it0))
+    {{fun _ s => P tt s /\ (cond s) = false}}.
+  Admitted. *)
+
+Definition slow_add (m : nat) : State MySt unit :=
+  for i = m to 0 {{
+    add_s m
+  }}.
+
+(* Definition fast_add : State unit :=
+  for i = 5 to 0 {{
+    add_s i
+  }}. *)
+
+Definition compare : State MySt bool :=
+  perf s <- (@get MySt) ;
+  state_pure (Nat.leb (r s) 2).
+
+(* Definition parity_x : State unit :=
+  for_e i = 500 to 0 {{
+    perf cond <- compare;
+    if (cond) then break
+    else loopT_liftT(min_s 2)
+  }}.
+ *)
+(* Compute runState parity_x {| r := 10 |}. *)
+
+(* Lemma l_parity_x :
+  {{(fun s : St => r s = 10)}} parity_x {{(fun (_ : unit ) (s : St) => r s = 2)}}.
+  Admitted. *)
+(* Lemma foreach_rule (min max : nat) (P : () -> St -> Prop) (body : nat -> State ())
+  : (forall (it : nat), {{fun s => P tt s /\ (min <= it <= max)}} body it {{P}}) -> 
+    {{P tt}} foreach max min (fun it0 => loopT_liftT (body it0)) {{fun _ s => P tt s}}. *)
+Lemma l_slow_add (m : nat) : 
+ {{(fun s : MySt => True)}} slow_add m{{(fun (_ : unit ) (s : MySt) => r s >= m)}}.
+  Proof.
+  unfold slow_add.
+  eapply weaken.
+(*   eapply strengthen. *)
+  apply foreach_rule.
+  unfold add_s.
+  intros.
+  eapply weaken.
+  apply l_modify.
+  simpl.
+  intros.
+  auto.
+  simpl.
+  intros.
+  auto.
+  Admitted.
+
+Fixpoint sumsum (n : nat): nat :=
+  match n with
+    | 0 => 0
+    | S n' => n + (sumsum n')
+  end.
+  
+(* Lemma l_fast_add (n : nat):
+  {{(fun s : St => r s = n)}} fast_add {{(fun (_ : unit ) (s : St) => r s < (Nat.add (sumsum 5) n))}}.
+  Proof.
+  apply weaken with (fun s => r s <= 42).
+  eapply strengthen.
+  apply foreach_rule. *)
+
+End ResNat.
+
+Section ResTab.
+
+Axiom tableSize : nat.
+Axiom maxTimeOut : nat.
+
+
+Axiom tableSizeNotZero : tableSize > 0.
+Axiom timeOutNotZero : maxTimeOut > 0.
+Axiom timeOutBiggerTableSize : tableSize < maxTimeOut.
+
+(* Definition tableSize := 10. *)
+
+(* Record index := {
+  i :> nat ;
+  Hi : i < tableSize }. *)
+
+Record tab : Type := {
+  mytab : list nat
+}.
+
+Definition addElement (n : nat) : State tab unit :=
+  modify (fun s => {| mytab := n :: (mytab s)|}).
+
+Lemma LaddElement (n : nat) (P : unit -> tab -> Prop) :
+{{fun  s => P tt {| mytab := n :: (mytab s) |} }} addElement n {{P}}.
+Proof.
+unfold addElement.
+eapply weaken.
+eapply l_modify.
+intros.
+simpl.
+assumption.
+Qed.
+
+Definition initT0 : State tab unit :=
+  for i = tableSize to 0 {{
+    addElement 0
+  }}.
+
+Definition readTabEntry (idx : nat) (ltab : tab) : nat :=
+  nth idx (mytab ltab) 0.
+
+(* Definition goodInitT0 (l : tab) :=
+  exists i : nat, length (mytab l) = i /\ (readTabEntry i l = 0). *)
+
+(* Lemma LAddElement (i : length) (P : unit -> tab -> Prop) :
+  {{fun s => P tt s /\ }} addElement 0 *)
+
+(* Lemma LinitT0 (P : unit -> tab -> Prop) :
+  {{fun s => P tt s /\ goodInitT0 s}} initT0 {{fun _ s => P tt s /\ goodInitT0 s}}.
+  Proof.
+  unfold initT0.
+  apply foreach_rule.
+  + intros it s H.
+    apply LaddElement.
+    intuition.
+    -  
+  Qed. *)
+
+Fixpoint changeElement (i n : nat) (l: list nat) : list nat :=
+ match (l,i) with
+  | ([], _) => []
+  | (a :: l', 0) => n :: l'
+  | (a :: l', S i') => a :: changeElement i' n l'
+  end.
+
+Definition changeTab (i n: nat) : State tab unit :=
+  modify (fun s => {| mytab := changeElement i n (mytab s)|}).
+
+Definition init_table (size : nat) : State tab unit :=
+  for i = size to 0 {{
+    changeTab (i-1) i 
+  }}.
+
+(* Definition init_table (size : nat) : State tab unit :=
+(*   initT0 ;; *)
+  init_table_aux size. *)
+
+(* Compute runState init_table {| mytab := [] |}. *)
+
+Definition goodInitT0 (size : nat) (l : tab) : Prop := 
+  length (mytab l) = size /\ (forall i : nat, 0 <= i < size /\ (readTabEntry i l = 0)).
+
+Definition goodInitTable (size : nat) (l : tab) : Prop :=
+  length (mytab l) = size /\ (forall i : nat, 0 <= i < size /\ (readTabEntry i l = i + 1 )).
+
+(* Definition invariantTable (i :  (l : tab) : Prop *)
+
+Lemma initPEntry (size : nat)  :
+  {{fun (s : tab) => goodInitT0 size s}} init_table size {{fun _ s => goodInitTable size s}}.
+  Proof.
+  unfold init_table.
+  unfold foreach.
+  revert size.
+  induction size.
+  +  intros s_init [HInit1 HInit2]. unfold foreach.
+     edestruct HInit2 as [H1 H2].
+     intuition ; omega.
+  + case_eq (S size <=? 0).
+    - intros.
+      apply ret.
